sintaxa.v
@@ -1,0 +1,427 @@
+(*SYNTAX*)
+
+(*Variables and environment*)
+
+
+Require Import Strings.String.
+Local Open Scope string_scope.
+Local Open Scope list_scope.
+Scheme Equality for string.
+Require Import Coq.Lists.List.
+Import ListNotations.
+Scheme Equality for list.
+
+Inductive ErrorNat :=
+  | error_nat : ErrorNat
+  | num : nat -> ErrorNat.
+
+Inductive ErrorBool :=
+  | error_bool : ErrorBool
+  | boolean : bool -> ErrorBool.
+
+Inductive ErrorString := 
+| error_string : ErrorString
+| String : string -> ErrorString.
+
+Coercion num: nat >-> ErrorNat.
+Coercion boolean: bool >-> ErrorBool.
+Coercion String : string >-> ErrorString.
+Scheme Equality for ErrorNat.
+Scheme Equality for ErrorString.
+Scheme Equality for ErrorBool.
+
+(* Arithmetic expressions *)
+
+ Inductive AExp :=
+| avar : string -> AExp
+| anum : ErrorNat -> AExp
+| aplus : AExp -> AExp -> AExp
+| amin : AExp -> AExp -> AExp
+| amul : AExp -> AExp -> AExp
+| adiv : AExp -> AExp -> AExp
+| amod : AExp -> AExp -> AExp
+| slength: ErrorString -> AExp.
+
+
+Coercion avar : string >-> AExp.
+Coercion anum : ErrorNat >-> AExp.
+Notation "A +' B" := (aplus A B)(at level 50, left associativity).
+Notation "A -' B" := (amin A B)(at level 50, left associativity).
+Notation "A *' B" := (amul A B)(at level 48, left associativity).
+Notation "A /' B" := (adiv A B)(at level 48, left associativity).
+Notation "A %' B" := (amod A B)(at level 45, left associativity).
+Notation "len( A )" := (slength A) (at level 50, left associativity).
+
+(* Boolean expressions *)
+
+Inductive BExp :=
+| berror: BExp
+| btrue : BExp
+| bfalse : BExp
+| bvar : string -> BExp
+| bnot : BExp -> BExp
+| band : BExp -> BExp -> BExp
+| bor : BExp -> BExp -> BExp
+| blessthan : AExp -> AExp -> BExp
+| bgreaterthan : AExp -> AExp -> BExp
+| isPrefix: ErrorString -> ErrorString -> BExp.
+
+Notation "A <' B" := (blessthan A B) (at level 72).
+Notation "A >' B" := (bgreaterthan A B) (at level 70).
+Notation "!' A" := (bnot A)(at level 50).
+Infix "and'" := band (at level 80).
+Infix "or'" := bor (at level 80).
+
+(* String operations*)
+
+ Inductive StringExp :=
+| svar : string -> StringExp
+| sstring : ErrorString -> StringExp
+| strcat: StringExp -> StringExp -> StringExp
+| areEqual: StringExp -> StringExp -> StringExp
+| substring: StringExp -> nat -> nat -> StringExp.
+
+
+Coercion svar: string >->StringExp.
+Notation " A += B " := (strcat A B) (at level 60). 
+
+Notation "A /in B" := (substring A B)(at level 55).
+
+
+Check "ana" += "maria". 
+
+
+
+(* pointers and references*)
+
+Inductive pointer := 
+| nullptr : pointer
+| ptr : string -> pointer
+| ref : string -> pointer.
+Scheme Equality for pointer.
+(* In c++ references are an alternative name for the same variable, and a pointer is a variable that,
+instead of data, it stores adresses *)
+(* in C un pointer poate fi asignat/declarat doar cu trei tipuri de valori: un alt pointer, referinta unei variabile
+sau NULL*)
+Notation " A **" := (ptr A)(at level 20).
+Notation "&& A" := (ref A )(at level 20).
+Check "a"**.
+Check &&"a".
+
+(*Arrays*)
+
+Inductive Array :=
+| error_array
+| array_nat : string ->nat -> list nat -> Array
+| array_bool : string -> nat -> list bool -> Array
+| array_string : string -> nat -> list string -> Array.
+
+Notation "A [[ N ]]->n B  " := (array_nat A N B) (at level 50).
+Notation "A [[ N ]]->b B " := (array_bool A N B) (at level 50).
+Notation "A [[ N ]]->s B  " := (array_string A N B) (at level 50).
+
+Check "a"[[10]]->n [ 1;2;3].
+
+Inductive ArrayExp :=
+| arr_const: Array->ArrayExp
+| arr_var: string -> ArrayExp
+| elementAt : Array -> nat ->ArrayExp
+| first: Array -> ArrayExp
+| last: Array -> ArrayExp 
+| deleteAt: Array -> nat -> ArrayExp
+| insertNat: Array  -> nat -> ArrayExp
+| insertBool: Array  -> bool -> ArrayExp
+| insertString: Array  -> string -> ArrayExp.
+
+Notation " s [[' i ']] " := (elementAt s i)(at level 22).
+
+Check ("a"[[10]]->n [1;2;3])[['1']].
+
+(* List Operations *)
+
+Inductive ListTypes :=
+| natList: list nat -> ListTypes
+| boolList: list bool -> ListTypes
+| stringList: list string -> ListTypes.
+
+Notation "l->n A" := (natList A)(at level 38).
+Notation "l->b A" := (boolList A)(at level 38).
+Notation "l->s A" := (stringList A)(at level 38).
+Check l->n [1;2;3].
+Check l->b [true;false].
+Check l->s ["mama";"tata"].
+
+Inductive ListElmType :=
+| natElm : nat -> ListElmType
+| boolElm : bool -> ListElmType
+| stringElm : string -> ListElmType.
+
+Coercion natElm: nat >-> ListElmType.
+Coercion boolElm: bool >-> ListElmType.
+Coercion stringElm: string >-> ListElmType.
+
+Inductive ListOp :=
+| List : ListTypes -> ListOp
+| listvar : string -> ListTypes -> ListOp
+| begin : ListOp -> ListOp
+| End' : ListOp -> ListOp
+| push_front : ListOp -> ListElmType -> ListOp
+| push_back : ListOp -> ListElmType -> ListOp
+| pop_front : ListOp -> ListOp
+| pop_back : ListOp -> ListOp.
+
+Notation "A <op>" := (List A) (at level 36).
+Notation "A .begin()" := (begin A) (at level 50).
+Notation "A .End()" := (End' A) (at level 50).
+Notation "A .push_front( B )" := (push_front A B) (at level 50).
+Notation "A .push_back( B )" := (push_front A B) (at level 50).
+Notation "A .pop_front()" := (pop_front A) (at level 50).
+Notation "A .pop_back()" := (pop_back A) (at level 50).
+Check (l->n [1;2;3]) <op>.
+Check ((l->n [1;2;3]) <op>).begin().
+Check ((l->n [1;2;3]) <op>).End().
+Check ((l->n [1;2;3]) <op>).push_back(natElm 1).
+
+
+
+
+(*Statements*)
+
+Inductive Stmt :=
+| error_stmt
+| nat_decl : string -> AExp -> Stmt
+| bool_decl : string -> BExp -> Stmt
+| string_decl : string -> StringExp -> Stmt
+| array_decl : Array  -> Stmt
+| pointer_decl: string -> pointer -> Stmt
+| reference_decl : string -> string -> Stmt
+| list_decl : string -> ListOp -> Stmt
+| struct_decl : string -> string -> Stmt
+| nat_assign : string -> AExp -> Stmt
+| bool_assign : string -> BExp -> Stmt
+| string_assign : string -> StringExp -> Stmt
+| pointer_assign : string -> pointer -> Stmt
+| reference_assign : string -> string -> Stmt
+| sequence : Stmt -> Stmt -> Stmt
+| ifthen : BExp -> Stmt -> Stmt
+| ifthenelse : BExp -> Stmt -> Stmt -> Stmt
+| while : BExp -> Stmt -> Stmt
+| For : Stmt -> BExp -> Stmt -> Stmt -> Stmt
+| switch : AExp -> list cases -> Stmt
+| functionCall: string -> list parameters -> Stmt
+with cases  :=
+| case : AExp -> Stmt -> cases
+| defaultcase: Stmt -> cases
+with parameters :=
+| error_param
+| nat_param :  ErrorNat -> parameters
+| bool_param : ErrorBool -> parameters
+| string_param : ErrorString -> parameters
+| variable : string -> parameters.
+
+
+Notation "'Nat'' X ::= A" := (nat_decl X A)(at level 90).
+Notation "'Bool' X ::= A" := (bool_decl X A)(at level 90).
+Notation "'Stringg' X ::= A" := (string_decl X A)(at level 92).
+Notation "Array'::= A" := (array_decl A ) (at level 58). 
+Notation "A ::p= B" := (pointer_decl A B) (at level 59).
+Notation "A ::r= B" := (reference_decl A B) (at level 50).
+Notation "A ::l= B" := (list_decl A B) (at level 60).
+Notation "X :n= A" := (nat_assign X A)(at level 90).
+Notation "X :b= A" := (bool_assign X A)(at level 90).
+Notation "X :s= A" := (string_assign X A)(at level 90).
+Notation "X :p= A" := (pointer_assign X A)(at level 80).
+Notation "X :r= A" := (reference_assign X A)(at level 80).
+Notation "S1 ;; S2" := (sequence S1 S2) (at level 98).
+Notation "'If' B 'Then' S1 'End'" := (ifthen B S1) (at level 97).
+Notation "'If' B 'Then' S1 'Else' S2 'End'" := (ifthenelse B S1 S2) (at level 97).
+Notation "'For(' S1 ';' B ';' S2 ')' '{' S3 '}'" := (For S1 B S2 S3)(at level 88).
+Notation "F  {{ A }}  " :=  (functionCall F A)(at level 88).
+
+Check "a" ::p= nullptr.
+Check "a" ::p= ("b" **).
+Check "a" ::p= (&& "b").
+Check "list1" ::l= (l->n [1;2;3]) <op>.
+Check "a" :n= 0.
+Check Nat' "a" ::= 0.
+Check Stringg "a" ::=  "ana".
+Check If "b">'2 Then "a" ::p= &&"b" End.
+Check If "b">'2 Then "a" ::p= &&"b" Else "a" ::p= nullptr End.
+Check For("a":n=0 ; "a"<'10 ; "a" :n= "a" +' 1)
+{
+   "s" :n= "s" +' "a"
+ }.
+Check "a" :p= nullptr.
+Check Array'::= "a" [[10]]->n [1;2].
+Check "func" {{[variable "a"]}}.
+Check switch (1+'2) [ defaultcase ("a" :n= 5)].
+Check switch (avar "a")
+    [case (5) ("a" :n= 4);
+     defaultcase ("a" :n= 0)].
+Compute  nth 1 [case (5) ("a" :n= 4); defaultcase ("a" :n= 0)].
+Compute List.last (rev [1;2;3]).
+
+Inductive types :=
+| error_types
+| naturalT: string -> types
+| booleanT: string -> types
+| StringT: string -> types.
+
+Inductive Value:=
+| undeclared : Value
+| default : Value
+| default_nat : Value
+| default_bool : Value
+| default_string : Value
+| err_assign : Value
+| nat_value : ErrorNat -> Value
+| bool_value : ErrorBool -> Value
+| string_value : ErrorString -> Value
+| array_value: Array -> Value
+| list_value: ListOp -> Value
+| code : Stmt -> Value.
+
+
+Definition Value_equality (t1 : Value) (t2 : Value) : bool :=
+  match t1 with
+    | undeclared => match t2 with 
+                     | undeclared => true
+                     | _ => false
+                     end
+    | default => match t2 with 
+                  | default => true
+                  | _ => false
+                  end
+    | default_nat => match t2 with
+                  | default => true
+                  | _ => false
+                  end
+    | default_bool => match t2 with
+                  | default_bool => true
+                  | _ => false
+                  end
+    | default_string => match t2 with
+                  | default_string => true
+                  | _ => false
+                  end
+    | err_assign => match t2 with 
+                  | err_assign => true
+                  | _ => false
+                  end
+    | nat_value a => match t2 with
+                  | nat_value b => if (ErrorNat_beq a b) then true else false
+                  | _ => false
+                  end
+    | bool_value a => match t2 with 
+                  | bool_value b => if (ErrorBool_beq a b) then true else false
+                  | _ => false
+                  end
+    | string_value  a => match t2 with
+                  | string_value b => if (ErrorString_beq a b) then true else false
+                  | _ => false
+                  end
+    | array_value  _x => match t2 with
+                  | array_value _x => true
+                  | _ => false
+                  end
+    | list_value  _x => match t2 with
+                  | list_value _x => true
+                  | _ => false
+                  end
+    | code _x => match t2 with
+                  | code _x => true
+                  | _ => false
+                 end
+  end. 
+
+Check code ("a" :n= 0).
+Inductive  members :=
+| member: string -> Value -> members.
+
+Definition FunctionEnv := string -> list types.
+Definition StructEnv := string -> list members.
+Definition functionEnv : FunctionEnv :=
+  fun x => [].
+Definition structEnv : StructEnv :=
+  fun x => [].
+Definition update_FunctionEnv (fnc_env:FunctionEnv) (s:string) (l:list types) : FunctionEnv :=
+ fun x => 
+     if (string_beq s x) then l
+     else (fnc_env x).
+
+Definition update_StructEnv (st_env:StructEnv) (s:string) (l:list members) :StructEnv :=
+  fun x =>
+      if (string_beq s x) then l
+      else (st_env x).
+(* Program *)
+
+Inductive program :=
+| Seq_prg: program -> program -> program
+| decl_globalNat : string -> AExp -> program
+| decl_globalBool : string -> BExp -> program
+| decl_globalString : string -> StringExp -> program
+| function: string -> list types -> Value -> program
+| struct : string -> list members -> program
+| main: Stmt ->program.
+
+Notation " A ;;; B " := (Seq_prg A B)(at level 20).
+Notation "'Nat_gl' A ::n= B" := (decl_globalNat A B)(at level 30).
+Notation "'Bool_gl' A ::b= B" := (decl_globalBool A B)(at level 30).
+Notation "'String_gl' A ::s= B" := (decl_globalString A B)(at level 30).
+(* Notation "'func' A '(' B ')' '{(' C ')}' 'end_func'" := (function A B C)(at level 30). *)
+
+Check main ("a" :n= 10) ;;; function "f1" [naturalT "a"] (code ("a" :n=10)).
+Check Nat_gl "a" ::n= 10.
+Check Bool_gl "b" ::b= btrue.
+Check String_gl "s" ::s= "start"%string.
+
+
+Check "n" :n= 10 ;;
+      "ok" :b= btrue ;;
+      "i" :n= 0 ;;
+      "msg" :s= "Hello" ;;
+
+      "func" {{[variable "a"]}};;
+      switch (avar "a")
+     [case (5) ("a" :n= 4);
+     defaultcase ("a" :n= 0)];;
+      while ("i" <' "n" +' 1) (
+            "s" :n= "s" +' 1 ;;
+            "i" :n= "i" +' 1
+      ).
+
+Definition prg := 
+  (Nat_gl "sum" ::n= 0) ;;;
+  function "suma" [naturalT "a"]
+  (
+   code(
+    For("i":n=0 ; "i"<'"a" ; "i" :n= "i" +' 1)
+    {
+     "sum" :n= "sum" +' "a"
+    }
+  )
+  ) ;;;
+  (struct "pereche"
+  [
+    member "stanga" default_nat;
+    member "dreapta" default_nat
+  ]);;;
+
+  main 
+      (Nat' "a" ::= 10 ;;
+      "ok" :b= btrue ;;
+      "i" :n= 0 ;;
+      "msg" :s= "Hello" ;;
+      "nume" :s= "Ana" += "Maria" ;;
+      "suma" {{[variable "a"]}};;
+      switch (avar "a")
+     [case (5) ("a" :n= 4);
+     defaultcase ("a" :n= 0)];;
+      while ("i" <' "n" +' 1) (
+            "s" :n= "s" +' 1 ;;
+            "i" :n= "i" +' 1
+      )
+).
+Compute prg.
+
+
